codes/PTSSignatureOps.v
@@ -1,0 +1,21 @@
+Require Import Thesis.PTSSignature.
+
+Module DisjointUnion (Sig1 Sig2 : PTS_SIGNATURE) <: PTS_SIGNATURE.
+
+  Definition Sort := (Sig1.Sort + Sig2.Sort)%type.
+
+  Definition A (x y : Sort) : Prop :=
+    match x, y with
+    | inl x1, inl y1 => Sig1.A x1 y1
+    | inr x2, inr y2 => Sig2.A x2 y2
+    | _, _ => False
+    end.
+
+  Definition R (x y z : Sort) : Prop :=
+    match x, y, z with
+    | inl x1, inl y1, inl z1 => Sig1.R x1 y1 z1
+    | inr x2, inr y2, inr z2 => Sig2.R x2 y2 z2
+    | _, _, _ => False
+    end.
+
+End DisjointUnion.
